StoreAtomicity.v
@@ -7,14 +7,14 @@ Record StoreAtomic (respFn: nat -> option Resp) :=
     uniqRespLabels:
       forall t1 t2, match respFn t1, respFn t2 with
                       | Some (Build_Resp c1 i1 _), Some (Build_Resp c2 i2 _) =>
-                        c1 = c2 -> i1 = i2 -> t1 = t2
+                        p_node c1 = p_node c2 -> i1 = i2 -> t1 = t2
                       | _, _ => True
                     end;
 
     localOrdering:
       forall t1 t2, match respFn t1, respFn t2 with
                       | Some (Build_Resp c1 i1 _), Some (Build_Resp c2 i2 _) =>
-                        c1 = c2 -> i1 > i2 -> t1 > t2
+                        p_node c1 = p_node c2 -> i1 > i2 -> t1 > t2
                       | _, _ => True
                     end;
 
@@ -24,7 +24,7 @@ Record StoreAtomic (respFn: nat -> option Resp) :=
                      forall i1, i1 < i2 -> exists t1, t1 < t2 /\
                                                       match respFn t1 with
                                                         | Some (Build_Resp c1 i _) =>
-                                                          c1 = c2 /\ i = i1
+                                                          p_node c1 = p_node c2 /\ i = i1
                                                         | None => False
                                                       end
                    | _ => True
