Makefile
@@ -1,6 +1,3 @@
-#MODULES := Rules Cache Channel Compatible DataTypes Hier L1 LatestValue MsiState StoreAtomicity Tree Useful Top L1Axioms LatestValueAxioms ChannelAxiom ChannelAxiomHelp CompatBehavior ChannelAxiomHelp HierProperties BehaviorAxioms BaseTree Case
-#VS      := $(MODULES:%=%.v)
-
 IGNORE:=
 
 VS:=$(wildcard *.v)
